main/Semantics.v
@@ -4,96 +4,80 @@ Require Import List.
 
 Require Import main.Syntax.
 
-Open Scope list_scope.
-
-
-(* TODO: Move to Proofs *)
-Let fn_vars := "fa"%string :: nil.
-Let fn_code := Declare_Aexp fn_vars  :: nil.
-Let fname := "called_fn"%string.
-Definition cc_funs_env := defineFunction Empty_Functions_Env fname (Body fn_code).
-
-
-Let calling_contract := Default_ContractState.
-Let called_addr := "called_contract"%string.
-Let called_contract := mkContractState called_addr true cc_funs_env Empty_Aexp_Env Empty_Bexp_Env.
-
-
-Definition c_env (addr : address) : ContractState :=
-match addr with
-| called_addr => called_contract
-end.
+Open Scope string_scope.
 
 
 Definition EnvStack := list (FunctionEnv * ContractState).
 
-Definition ExecutionState : Type :=  Code * FunctionEnv * EnvStack * ContractState.
+Definition ExecutionState : Type :=  Code * FunctionEnv * EnvStack * ContractState * ContractsEnv.
+
+Open Scope list_scope.
 
 Inductive step : ExecutionState -> ExecutionState -> Prop :=
 | transfer:
-    forall dest_addr amount value final_bm rest fenv env_stack c_st new_bm src_addr old_bm,
+    forall dest_addr amount value final_bm rest fenv env_stack c_st c_env new_bm src_addr old_bm,
       src_addr = (c_address c_st) ->
       old_bm = (balance_map fenv) ->
       value = unfoldOptionZ (evalaexp (aexp_env fenv) amount) ->
       new_bm = (updateBalance old_bm dest_addr ((old_bm dest_addr) + value)) ->
       final_bm = (updateBalance new_bm src_addr ((new_bm src_addr) - value)) ->
-      step (Transfer dest_addr amount :: rest, fenv, env_stack, c_st)
+      step (Transfer dest_addr amount :: rest, fenv, env_stack, c_st, c_env)
            (rest,
            mkEnv (aexp_env fenv) (bexp_env fenv) rest final_bm (msg_data fenv),
            env_stack,
-           c_st)
+           c_st, c_env)
 
 | function_call:
-    forall called_addr msg_val value env env_stack c_st c_st' fenv fcode fname rest,
+    forall called_addr msg_val value env env_stack c_st c_env c_st' fenv fcode fname rest,
       c_st' = c_env called_addr ->
       fcode = getFunctionCode ((fn_env c_st') fname) ->
       value = unfoldOptionZ (evalaexp (aexp_env env) msg_val) ->
       fenv = mkEnv (Empty_Aexp_Env) (Empty_Bexp_Env) (rest) (balance_map env) (mkMsg value (c_address c_st)) ->
-      step ((Function_Call called_addr fname msg_val) :: rest, env, env_stack, c_st) (fcode, fenv, (env, c_st) :: env_stack, c_st')
+      step ((Function_Call called_addr fname msg_val) :: rest, env, env_stack, c_st, c_env) (fcode, fenv, (env, c_st) :: env_stack, c_st', c_env)
 
 | function_exit:
-    forall (fenv fenv' : FunctionEnv) (c_st c_st' : ContractState) env_stack,
-      step (nil, fenv, (fenv', c_st') :: env_stack, c_st)
-           (next_code fenv', fenv', env_stack, c_st')
+    forall (fenv fenv' : FunctionEnv) (c_st c_st' : ContractState) env_stack c_env,
+      step (nil, fenv, (fenv', c_st') :: env_stack, c_st, c_env)
+           (next_code fenv', fenv', env_stack, c_st', c_env)
 
 | skip:
-    forall rest env env_stack c_st,
-      step (Skip :: rest, env, env_stack, c_st) (rest, env, env_stack, c_st)
+    forall rest env env_stack c_st c_env,
+      step (Skip :: rest, env, env_stack, c_st, c_env) (rest, env, env_stack, c_st, c_env)
 
 | declare_aexp:
-    forall aexp_env' aexp_names rest env env' env_stack c_st,
+    forall aexp_env' aexp_names rest env env' env_stack c_st c_env,
       aexp_env' = declareAexpList (aexp_env env) aexp_names ->
       env' = mkEnv aexp_env' (bexp_env env) (next_code env) (balance_map env) (msg_data env) ->
-      step ((Declare_Aexp aexp_names) :: rest, env, env_stack, c_st) (rest, env', env_stack, c_st)
+      step ((Declare_Aexp aexp_names) :: rest, env, env_stack, c_st, c_env) (rest, env', env_stack, c_st, c_env)
 
 | assign_aexp : 
-    forall a x v aexp_env' rest env env' env_stack c_st,
+    forall a x v aexp_env' rest env env' env_stack c_st c_env,
       v = unfoldOptionZ (evalaexp (aexp_env env) a) ->
       aexp_env' = updateAexp (aexp_env env) x v ->
       env' = mkEnv aexp_env' (bexp_env env) (next_code env) (balance_map env) (msg_data env) ->
-      step (Assignment_Aexp x a :: rest, env, env_stack, c_st) (rest, env', env_stack, c_st)
+      step (Assignment_Aexp x a :: rest, env, env_stack, c_st, c_env) (rest, env', env_stack, c_st, c_env)
 
 | assign_bexp :
-    forall b x v bexp_env' rest env env' env_stack c_st,
+    forall b x v bexp_env' rest env env' env_stack c_st c_env,
       v = unfoldOptionBool (evalbexp (aexp_env env) (bexp_env env) b) ->
       bexp_env' = updateBexp (bexp_env env) x v ->
       env' = mkEnv (aexp_env env) (bexp_env') (next_code env) (balance_map env) (msg_data env) ->
-      step (Assignment_Bexp x b :: rest, env, env_stack, c_st) (rest, env', env_stack, c_st)
+      step (Assignment_Bexp x b :: rest, env, env_stack, c_st, c_env) (rest, env', env_stack, c_st, c_env)
 
 | if_true :
-    forall b s1 s2 rest env env_stack c_st,
+    forall b s1 s2 rest env env_stack c_st c_env,
       Some true = (evalbexp (aexp_env env) (bexp_env env) b) ->
-      step (IfThenElse b s1 s2 :: rest, env, env_stack, c_st) (s1 ++ rest, env, env_stack, c_st)
+      step (IfThenElse b s1 s2 :: rest, env, env_stack, c_st, c_env) (s1 ++ rest, env, env_stack, c_st, c_env)
 
 | if_false :
-    forall b s1 s2 rest env env_stack c_st,
+    forall b s1 s2 rest env env_stack c_st c_env,
       Some false = (evalbexp (aexp_env env) (bexp_env env) b) ->
-      step (IfThenElse b s1 s2 :: rest, env, env_stack, c_st) (s2 ++ rest, env, env_stack, c_st)
+      step (IfThenElse b s1 s2 :: rest, env, env_stack, c_st, c_env) (s2 ++ rest, env, env_stack, c_st, c_env)
 
 | while:
-    forall (s : list instr) b rest env env_stack c_st,
-      step (While b s :: rest, env, env_stack, c_st)
-           ((IfThenElse b (s ++ While b s :: nil) (Skip :: nil)) :: rest, env, env_stack, c_st)
+    forall (s : list instr) b rest env env_stack c_st c_env,
+      step (While b s :: rest, env, env_stack, c_st, c_env)
+           ((IfThenElse b (s ++ While b s :: nil) (Skip :: nil)) :: rest, env, env_stack, c_st, c_env)
 .
 
 Inductive steps : ExecutionState -> ExecutionState -> Prop :=
@@ -103,17 +87,22 @@ Inductive steps : ExecutionState -> ExecutionState -> Prop :=
     step S S' -> steps S' S'' -> steps S S''.
 
 
-
 (* Examples *)
 
-Let receiver := "addr"%string.
-Let amount := Int 1%Z.
+
+(** address.transfer(amount) *)
+
+Let receiver := "addr".
+Let amount := Int 1.
 Let amount_z := 1%Z.
 
-(* Example for: address.transfer(amount) *)
+Let example_contracts_env := Empty_ContractsEnv.
+
 Example transfer_ex:
-  steps (Transfer receiver amount :: nil, Empty_FunctionEnv, nil, Default_ContractState)
-        (nil, replace_bmap Empty_FunctionEnv (updateBalance (updateBalance Empty_BalanceMap receiver amount_z) (c_address Default_ContractState) (-amount_z)), nil, Default_ContractState)
+  steps (Transfer receiver amount :: nil, Empty_FunctionEnv, nil, Default_ContractState, example_contracts_env)
+        (nil, replace_bmap Empty_FunctionEnv 
+        (updateBalance (updateBalance Empty_BalanceMap receiver amount_z) 
+        (c_address Default_ContractState) (-amount_z)), nil, Default_ContractState, example_contracts_env)
   .
 Proof.
   eapply trans.
@@ -127,20 +116,30 @@ Proof.
 
 
 
-Let msg_val := Int 0%Z.
+
+(** Setup *)
+Let called_fn_code := Declare_Aexp ("fn_a" :: nil)  :: nil.
+Let called_fn := "called_fn".
+Let called_contract_funs_env := defineFunction Empty_Functions_Env called_fn (Body called_fn_code).
+Let called_contract_address := "called_contract".
+Let called_contract_state := mkContractState called_contract_address called_contract_funs_env Empty_Aexp_Env Empty_Bexp_Env.
+
+Let calling_contract_state := Default_ContractState.
+
+Let example2_contracts_env := updateContractsEnv Empty_ContractsEnv called_contract_address called_contract_state.
+
+Let msg_val := Int 0.
 Let msg_val_z := 0%Z.
-Let current_vars := "a"%string :: nil.
-Let current_code := (Declare_Aexp current_vars) :: (Function_Call called_addr fname msg_val) :: nil.
+Let current_vars := "a" :: nil.
+Let current_code := (Declare_Aexp current_vars) :: (Function_Call called_contract_address called_fn msg_val) :: nil.
 
-Let initial_env := Empty_FunctionEnv.
-Let env_before_call := (replace_aexp_env initial_env (declareAexpList (aexp_env initial_env) current_vars)).
-Let called_fn_env := replace_msg_data initial_env (mkMsg  msg_val_z (c_address calling_contract)).
+Let fn_env_before_call := (replace_aexp_env Empty_FunctionEnv (declareAexpList (aexp_env Empty_FunctionEnv) current_vars)).
+Let called_fn_env := replace_msg_data Empty_FunctionEnv (mkMsg  msg_val_z (c_address calling_contract_state)).
 
-
-(* function call *)
+(** function call *)
 Example Step_Into_Call :
-  steps (current_code, initial_env, nil, calling_contract)
-        (fn_code, called_fn_env, (env_before_call, calling_contract) :: nil, called_contract).
+  steps (current_code, Empty_FunctionEnv, nil, calling_contract_state, example2_contracts_env)
+        (called_fn_code, called_fn_env, (fn_env_before_call, calling_contract_state) :: nil, called_contract_state, example2_contracts_env).
 Proof.
   eapply trans.
   - eapply declare_aexp; eauto.
@@ -150,81 +149,43 @@ Proof.
 Qed.
 
 
-(** Old, needs change *)
-(*
-Example Call_With_Code_After :
-  steps ((Declare_Aexp "n" :: nil) :: Function_Call "SUM" :: Assignment_Aexp "n" (Int 99) :: nil,
-   mkEnv Empty_Aexp_Env Empty_Bexp_Env fun_env nil,
-   nil)
-  (Assignment_Aexp "n" (Int 10) ::
-                   Assignment_Aexp "sum" (Int 0) ::
-                   While (Aexp_Geq (AId "n") (Int 1)) (
-                     Assignment_Aexp "sum" (Plus (AId "n") (AId "sum")) ::
-                     Assignment_Aexp "n" (Plus (AId "n") (Int (Z.opp 1))) :: nil
-                   ) :: nil,
-   mkEnv Empty_Aexp_Env Empty_Bexp_Env fun_env (Assignment_Aexp "n" (Int 99) :: nil),
-   (mkEnv (updateAexp (aexp_env Program_Env) "n" 1) Empty_Bexp_Env fun_env nil) :: nil).
+
+
+(** function exit *)
+
+Let fenv_with_remaining_code := replace_next_code Empty_FunctionEnv (Skip :: nil).
+Let called_contract_address2 := "called_contract".
+Let called_contract_state2 := mkContractState called_contract_address2 Empty_Functions_Env Empty_Aexp_Env Empty_Bexp_Env.
+
+Let calling_contract_state2 := Default_ContractState.
+
+Let example_contracts_env3 := updateContractsEnv 
+(updateContractsEnv Empty_ContractsEnv called_contract_address2 called_contract_state2)
+Default_Address calling_contract_state2.
+
+Example Function_exit:
+  steps (nil, Empty_FunctionEnv, (fenv_with_remaining_code, calling_contract_state2)::nil,
+  called_contract_state2, example_contracts_env3)
+  (next_code fenv_with_remaining_code, fenv_with_remaining_code, nil,
+   calling_contract_state2, example_contracts_env3).
 Proof.
-  apply trans with (S' := (Function_Call "SUM" :: Assignment_Aexp "n" (Int 99) :: nil,
-                          (mkEnv (updateAexp (aexp_env Program_Env) "n" 1) Empty_Bexp_Env fun_env nil),
-                          nil)).
-  -apply assign_aexp. simpl. reflexivity.
-  (* -apply trans with (S' := (Assignment_Aexp "n" (Int 10) :: nil,
-   mkEnv Empty_Aexp_Env Empty_Bexp_Env fun_env,
-   (mkEnv (updateAexp (aexp_env Program_Env) "n" 1) Empty_Bexp_Env fun_env) :: nil)). *)
-  -apply trans with (S' := (Assignment_Aexp "n" (Int 10) ::
-                   Assignment_Aexp "sum" (Int 0) ::
-                   While (Aexp_Geq (AId "n") (Int 1)) (
-                     Assignment_Aexp "sum" (Plus (AId "n") (AId "sum")) ::
-                     Assignment_Aexp "n" (Plus (AId "n") (Int (Z.opp 1))) :: nil
-                   ) :: nil,
-  mkEnv Empty_Aexp_Env Empty_Bexp_Env fun_env (Assignment_Aexp "n" (Int 99) :: nil),
-   (mkEnv (updateAexp (aexp_env Program_Env) "n" 1) Empty_Bexp_Env fun_env nil) :: nil)).
-    *apply function_call.
-     {
-      simpl. reflexivity.
-     }
-     {
-      simpl. reflexivity.
-     }
-    * apply refl.
+  eapply trans.
+  {
+    eapply function_exit; eauto.
+  }
+  {
+    apply refl.
+  }
   Qed.
 
-Example Step_Outside_Call :
-  steps (Assignment_Aexp "n" (Int 1) :: Function_Call "SUM" :: Assignment_Aexp "n" (Int 99) :: nil,
-   mkEnv Empty_Aexp_Env Empty_Bexp_Env fun_env nil,
-   nil)
-  (Assignment_Aexp "n" (Int 99) :: nil,
-   mkEnv (updateAexp (aexp_env Program_Env) "n" 1) Empty_Bexp_Env fun_env nil,
-   nil).
-Proof.
-  apply trans with (S' := (Function_Call "SUM" :: Assignment_Aexp "n" (Int 99) :: nil,
-                          (mkEnv (updateAexp (aexp_env Program_Env) "n" 1) Empty_Bexp_Env fun_env nil),
-                          nil)).
-  -apply assign_aexp. simpl. reflexivity.
-  (* -apply trans with (S' := (Assignment_Aexp "n" (Int 10) :: nil,
-   mkEnv Empty_Aexp_Env Empty_Bexp_Env fun_env,
-   (mkEnv (updateAexp (aexp_env Program_Env) "n" 1) Empty_Bexp_Env fun_env) :: nil)). *)
-  -apply trans with (S' := (Assignment_Aexp "n" (Int 10) ::
-                   Assignment_Aexp "sum" (Int 0) ::
-                   While (Aexp_Geq (AId "n") (Int 1)) (
-                     Assignment_Aexp "sum" (Plus (AId "n") (AId "sum")) ::
-                     Assignment_Aexp "n" (Plus (AId "n") (Int (Z.opp 1))) :: nil
-                   ) :: nil,
-  mkEnv Empty_Aexp_Env Empty_Bexp_Env fun_env (Assignment_Aexp "n" (Int 99) :: nil),
-   (mkEnv (updateAexp (aexp_env Program_Env) "n" 1) Empty_Bexp_Env fun_env nil) :: nil)).
-    *apply function_call.
-     {
-      simpl. reflexivity.
-     }
-     {
-      simpl. reflexivity.
-     }
-    * apply trans with (S' := (Assignment_Aexp "n" (Int 99) :: nil,
-   mkEnv (updateAexp (aexp_env Program_Env) "n" 1) Empty_Bexp_Env fun_env nil,
-   nil)).
-   { simpl. apply function_exit. reflexivity. }
-   { apply refl. }
-  Qed.
-  
-*)
+
+
+(** declare aexp in environment *)
+
+
+
+
+
+
+
+
